polymorphism/Proofs/Extended2_top.v
@@ -1,0 +1,1159 @@
+Require Import String.
+Require Import Coq.Structures.Equalities.
+Require Import Coq.MSets.MSetInterface.
+Require Import Arith.
+Require Import Setoid.
+Require Import Coq.Program.Equality.
+Require Import SystemF.
+Require Import Extended_definitions4_top.
+
+Module Extended
+       (Import VarTyp : UsualDecidableTypeFull)
+       (Import set : MSetInterface.S).
+
+(*
+Module Definitions := Definitions(VarTyp)(set).
+Import Definitions.
+*)
+Require Import Extended_infrastructure4_top.
+Module Infrastructure := Infrastructure(VarTyp)(set).
+Export Infrastructure.
+
+(* Notes:
+
+The syntax is encoded using Charguéraud's Locally nameless representation:
+
+http://www.chargueraud.org/softs/ln/
+
+We annotate the Coq theorems with the correnposing lemmas/theorems in the paper. 
+The reader can just look for:
+
+Lemma 4
+
+for example, to look for the proof of lemma 4 in the paper.
+
+All lemmas and theorems are complete: there are no uses of admit or Admitted,
+with the exceptions of "tlam" and "tylam" due to a technical limitation.
+
+*)
+
+
+Lemma ortho_ax_sym : forall A B, OrthoAx A B -> OrthoAx B A.
+Proof.
+  intros.
+  destruct H as [a [b c]].
+  unfold OrthoAx.
+  auto.
+Qed.
+  
+Lemma ortho_sym : forall Gamma A B, Ortho Gamma A B -> Ortho Gamma B A.
+Proof.
+  intros Gamma A B HOrtho.
+  induction HOrtho; auto.
+  - apply_fresh OForAll as x; apply H0; not_in_L x.
+  - apply OVarSym with (A := A); auto.
+  - apply OVar with (A := A); auto.
+  - apply ortho_ax_sym in H; now apply OAx.
+Qed.
+  
+Lemma ortho_and_l : forall Gamma t1 t2 t0, Ortho Gamma (And t1 t2) t0 -> Ortho Gamma t1 t0.
+Proof.
+  intros.
+  dependent induction H; auto.
+  - inversion H1; subst.
+    apply OVarSym with (A := A); auto.
+    apply sound_sub in H0.
+    destruct H0.
+    inversion H0; subst.
+    apply complete_sub.
+    eexists; apply H7.
+    inversion H3.
+    inversion H3.
+  - orthoax_inv_l.
+Qed.
+
+Lemma ortho_and_r : forall Gamma t1 t2 t0, Ortho Gamma (And t1 t2) t0 -> Ortho Gamma t2 t0.
+Proof.
+  intros.
+  dependent induction H; auto.
+  - inversion H1; subst.
+    apply OVarSym with (A := A); auto.
+    apply sound_sub in H0.
+    destruct H0.
+    inversion H0; subst.
+    apply complete_sub.
+    eexists; apply H9.
+    inversion H3.
+    inversion H3.
+  - orthoax_inv_l.
+Qed.
+
+Lemma wfenv_no_refl : forall Gamma x, WFEnv Gamma -> not (List.In (x, TyDis (PFVarT x)) Gamma).
+Proof.
+  intros.
+  induction H.
+  - auto.
+  - unfold not, extend; simpl in *; intros.
+    destruct H2.
+    inversion H2; subst.
+    apply H0; simpl.
+    now apply MSetProperties.Dec.F.singleton_2.
+    contradiction.
+  - unfold not, extend; simpl; intros [a | b]; apply IHWFEnv.
+    inversion a. auto.
+Qed.
+
+Lemma wfenv_no_var_sub :
+  forall Gamma x A, WFEnv Gamma -> Sub A (PFVarT x) -> not (List.In (x, TyDis A) Gamma).
+Proof.
+  intros.
+  induction H.
+  - auto.
+  - unfold not, extend; simpl in *; intros.
+    destruct H3.
+    inversion H3; subst.
+    inversion H0.
+    clear IHWFEnv H2 H0 H.
+    dependent induction H4.
+    + simpl in *; apply IHsub; not_in_L x.
+    + simpl in *; apply IHsub; not_in_L x.
+    + apply H1; simpl; now apply MSetProperties.Dec.F.singleton_2.
+    + contradiction.
+  - unfold not, extend; simpl; intros [a | b]; apply IHWFEnv.
+    inversion a. auto.
+Qed.
+
+Inductive TopLike : PTyp -> Prop :=
+  | TLTop : TopLike Top
+  | TLAnd : forall t1 t2, TopLike t1 -> TopLike t2 -> TopLike (And t1 t2)
+  | TLFun : forall t1 t2, TopLike t2 -> TopLike (Fun t1 t2) 
+  | TLForAll : forall L d t,
+                 (forall x, not (In x L) -> TopLike (open_typ_source t (PFVarT x))) ->
+                 TopLike (ForAll d t).
+
+Hint Constructors TopLike.
+
+Lemma toplike_dec : forall t, sumbool (TopLike t) (not (TopLike t)).
+Proof.
+  intro t.
+  induction t.
+  - right; unfold not; intros HInv; inversion HInv. 
+  - inversion IHt2.
+    left.
+    apply TLFun.
+    apply H.
+    right.
+    unfold not; intros HInv; inversion HInv; subst.
+    contradiction.
+  - destruct IHt1. destruct IHt2. left. apply TLAnd; auto.
+    right. unfold not. intros. inversion H; subst. contradiction.
+    destruct IHt2.
+    right. unfold not. intros. inversion H; subst. contradiction.
+    right. unfold not. intros. inversion H; subst. contradiction.
+  - right; unfold not; intros HInv; inversion HInv.
+  - right; unfold not; intros HInv; inversion HInv.
+  - right; unfold not; intros HInv; inversion HInv.
+    subst.
+    admit.
+  - left; apply TLTop.
+Admitted.
+
+Lemma ortho_no_sub :
+  forall Gamma A B, WFTyp Gamma A -> WFTyp Gamma B -> Ortho Gamma A B -> ~ TopLike B -> not (Sub A B).
+Proof.
+  intros Gamma A B WFA WFB HOrtho HNotTL HSub.
+
+  inversion HSub.
+  generalize dependent Gamma.
+  induction H; intros.
+  - inversion HOrtho; subst. destruct H as [a [b c]]; now apply c.
+  - inversion HOrtho; subst.
+    inversion WFA; inversion WFB; subst.
+    apply IHsub2 with (Gamma := Gamma); auto.
+    inversion HSub. inversion H1; subst.
+    eexists; apply H13.
+    destruct H1 as [a [b c]]; now apply c.
+  - inversion WFB; subst.
+    assert (Ha : ~ TopLike t1 \/ ~ TopLike t2).
+    apply Classical_Prop.not_and_or; unfold not; intros HH; destruct HH; auto.
+    destruct Ha.
+    apply IHsub1 with (Gamma := Gamma); auto.
+    eexists; apply H.
+    apply ortho_sym.
+    apply ortho_and_l with (t2 := t2); auto.
+    now apply ortho_sym.
+    apply IHsub2 with (Gamma := Gamma); auto.
+    eexists; apply H0.
+    apply ortho_sym.
+    apply ortho_and_r with (t1 := t1); auto.
+    now apply ortho_sym.    
+  - inversion WFA; subst; apply IHsub with (Gamma := Gamma); auto.
+    eexists; apply H.
+    apply ortho_and_l with (t2 := t2); auto.
+  - inversion WFA; subst; apply IHsub with (Gamma := Gamma); auto.
+    eexists; apply H.
+    apply ortho_and_r with (t1 := t1); auto.
+  - inversion HOrtho; subst.
+    apply wfenv_no_var_sub with (Gamma := Gamma) (A := A) (x := v); auto.
+    now apply wf_gives_wfenv in WFA.
+    now apply sound_sub.
+    apply wfenv_no_var_sub with (Gamma := Gamma) (A := A) (x := v); auto.
+    now apply wf_gives_wfenv in WFA.
+    now apply sound_sub.
+    destruct H as [a [b c]]; now apply c.    
+  - inversion WFA; inversion WFB; subst.
+    inversion HSub.
+    inversion H2; subst.
+    inversion HOrtho; subst.
+    pick_fresh x.
+    eapply H0 with (x := x).
+    not_in_L x.
+    unfold not; intros HH; apply HNotTL.
+    apply_fresh TLForAll as y.
+    admit. (* rename lemma fresh_bot? *)
+    eexists; apply H8.
+    not_in_L x.
+    apply H5.
+    not_in_L x.
+    apply H10.
+    not_in_L x.
+    apply H7.
+    not_in_L x.
+    destruct H3 as [a [b HH]]; now apply HH.
+  - auto.
+Admitted.
+
+Lemma usub_top : forall D, usub Top D -> TopLike D.
+  intros. dependent induction H. apply TLAnd; auto. apply TLTop.
+Defined.
+
+(* Unique subtype contributor: Lemma 2 *)
+
+Lemma uniquesub :
+  forall Gamma A B C, WFTyp Gamma A -> WFTyp Gamma B -> ~ TopLike C ->
+             Ortho Gamma A B -> Sub (And A B) C -> not (Sub A C /\ Sub B C).
+Proof.
+  intros Gamma A B C WFA WFB HNotTL HOrtho HSubAnd.
+  unfold not; intros [HSubA HSubB].
+  generalize dependent C.
+  dependent induction HOrtho; intros.
+  - induction C;
+    try now inversion WFA; subst;
+    inversion HSubA; inversion H; subst; [ eapply IHHOrtho1 | eapply IHHOrtho2 ];
+    unfold Sub; eauto.
+    + inversion HSubA; inversion H; subst.
+      inversion HSubB; inversion H0; subst.
+      assert (Ha : ~ TopLike C1 \/ ~ TopLike C2).
+      apply Classical_Prop.not_and_or; unfold not; intros HH; destruct HH; eauto.
+      destruct Ha.
+      apply IHC1; auto; unfold Sub; eauto.
+      apply sand2; unfold Sub; eauto.
+      apply IHC2; auto; unfold Sub; eauto.
+      apply sand2; unfold Sub; eauto.
+      inversion H2.
+      inversion H2.
+      inversion H3.
+      inversion H3.
+    + now apply HNotTL.
+  - induction C;
+    try now inversion WFB; subst;
+    inversion HSubB; inversion H; subst; [ eapply IHHOrtho1 | eapply IHHOrtho2 ];
+    unfold Sub; eauto.
+    + inversion HSubA; inversion H; subst.
+      inversion HSubB; inversion H0; subst.
+      assert (Ha : ~ TopLike C1 \/ ~ TopLike C2).
+      apply Classical_Prop.not_and_or; unfold not; intros HH; destruct HH; eauto.
+      destruct Ha.
+      apply IHC1; auto; unfold Sub; eauto.
+      apply sand2; unfold Sub; eauto.
+      apply IHC2; auto; unfold Sub; eauto.
+      apply sand2; unfold Sub; eauto.
+      inversion H6.
+      inversion H6.
+      inversion H1.
+      inversion H1.
+    + now apply HNotTL.
+  - induction C; try (now (inversion HSubA as [x HInv]; inversion HInv)).
+    + inversion WFA; subst; inversion WFB; subst.
+      inversion HSubA; inversion H; subst.
+      inversion HSubB; inversion H0; subst.
+      assert (Ha : ~ TopLike C2) by (unfold not; auto).
+      eapply IHHOrtho; auto; [ apply Ha
+                             | apply sand2; unfold Sub; eauto
+                             | unfold Sub; eauto
+                             | unfold Sub; eauto ].
+    + assert (Ha : ~ TopLike C1 \/ ~ TopLike C2).
+      apply Classical_Prop.not_and_or; unfold not; intros HH; destruct HH; eauto.
+      inversion WFA; subst; inversion WFB; subst.
+      inversion HSubA; inversion H; subst.
+      inversion HSubB; inversion H0; subst.
+      destruct Ha.
+      apply IHC1; unfold Sub; eauto.
+      apply sand2; unfold Sub; eauto.
+      apply IHC2; unfold Sub; eauto.
+      apply sand2; unfold Sub; eauto.
+    + now apply HNotTL.
+  - induction C; try (now (inversion HSubA as [x HInv]; inversion HInv)).
+    + inversion HSubA; inversion H1; subst.
+      inversion HSubB; inversion H2; subst.
+      assert (Ha : ~ TopLike C1 \/ ~ TopLike C2).
+      apply Classical_Prop.not_and_or; unfold not; intros HH; destruct HH; eauto.
+      destruct Ha.
+      apply IHC1; unfold Sub; eauto.
+      apply sand2; unfold Sub; eauto.
+      apply IHC2; unfold Sub; eauto.
+      apply sand2; unfold Sub; eauto.      
+    + inversion HSubA; inversion H1; subst.
+      inversion HSubB; inversion H2; subst.
+      inversion WFA; inversion WFB; subst.
+      pick_fresh x.
+      clear IHC1; clear IHC2; clear HSubAnd.
+      eapply H0 with (x := x) (C := open_typ_source C2 (PFVarT x)).
+      not_in_L x; apply H7.
+      apply H9; not_in_L x.
+      apply H15; not_in_L x.
+      admit. (* needs renaming lemma here *)
+      apply sand2.
+      eexists; apply H7.
+      not_in_L x.
+      apply wf_gives_types_source with (Gamma := (extend x (TyDis C1) Gamma)).
+      apply H15; not_in_L x.
+      eexists; apply H7; not_in_L x.
+      eexists; apply H6; not_in_L x.
+    + now apply HNotTL.
+  - induction C; try (now (inversion HSubA as [z HInv]; inversion HInv)).
+    + destruct HSubA as [c HsubA]; inversion HsubA; subst.
+      destruct HSubB as [c HsubB]; inversion HsubB; subst.
+      assert (Ha : ~ TopLike C1 \/ ~ TopLike C2).
+      apply Classical_Prop.not_and_or; unfold not; intros HH; destruct HH; eauto.
+      destruct Ha.
+      apply IHC1; unfold Sub; eauto.
+      apply sand2; unfold Sub; eauto.
+      apply IHC2; unfold Sub; eauto.
+      apply sand2; unfold Sub; eauto.
+      inversion H3.
+      inversion H3.
+    + clear HSubAnd.
+      destruct HSubA as [c HsubA]; inversion HsubA; subst.
+      assert (Ha : Ortho Gamma ty (PFVarT v)).
+      apply OVarSym with (A := A); auto.
+      apply ortho_no_sub in Ha.
+      contradiction.
+      auto.
+      auto.
+      unfold not; intros HInv; inversion HInv.
+    + now apply HNotTL.
+  (* same as above (var_sym) *)
+  - induction C; try (now (inversion HSubB as [z HInv]; inversion HInv)).
+    + destruct HSubA as [c HsubA]; inversion HsubA; subst.
+      destruct HSubB as [c HsubB]; inversion HsubB; subst.
+      assert (Ha : ~ TopLike C1 \/ ~ TopLike C2).
+      apply Classical_Prop.not_and_or; unfold not; intros HH; destruct HH; eauto.
+      destruct Ha.
+      apply IHC1; unfold Sub; eauto.
+      apply sand2; unfold Sub; eauto.
+      apply IHC2; unfold Sub; eauto.
+      apply sand2; unfold Sub; eauto.
+      inversion H3.
+      inversion H3.
+    + clear HSubAnd.
+      destruct HSubB as [c HsubB]; inversion HsubB; subst.
+      assert (Ha : Ortho Gamma ty (PFVarT v)).
+      apply OVarSym with (A := A); auto.
+      apply ortho_no_sub in Ha.
+      contradiction.
+      auto.
+      auto.
+      unfold not; intros HInv; inversion HInv.
+    + now apply HNotTL.
+  - apply complete_sub in HSubA; apply usub_top in HSubA; contradiction.
+  - apply complete_sub in HSubB; apply usub_top in HSubB; contradiction.
+  - destruct H as [ PTypHd1 [ PTypHd2 PTypHd3 ]].
+    induction C.
+    + inversion HSubA as [x HsA]; inversion HsA; subst; try orthoax_inv PTypHd1.
+      inversion HSubB as [x HsB]; inversion HsB; subst; try orthoax_inv PTypHd2.
+      apply PTypHd3; auto.
+    + inversion HSubA as [x HsA]; inversion HsA; subst; try orthoax_inv PTypHd1.
+      inversion HSubB as [x HsB]; inversion HsB; subst; try orthoax_inv PTypHd2.
+      apply PTypHd3; auto.
+    + inversion HSubA as [x HInv1]; inversion HInv1; subst; try (now inversion H0).
+      inversion HSubB as [x HInv2]; inversion HInv2; subst; try (now inversion H0).
+      assert (Ha : ~ TopLike C1 \/ ~ TopLike C2).
+      apply Classical_Prop.not_and_or; unfold not; intros HH; destruct HH; eauto.
+      destruct Ha.
+      apply IHC1; unfold Sub; eauto.
+      apply sand2; unfold Sub; eauto.
+      apply IHC2; unfold Sub; eauto.
+      apply sand2; unfold Sub; eauto.      
+    + inversion HSubA as [x HsA]; inversion HsA; subst; inversion H0.
+    + inversion HSubA as [x HsA]; inversion HsA; subst; try orthoax_inv PTypHd1.
+    + inversion HSubA as [x HsA]; inversion HsA; subst; try orthoax_inv PTypHd1.
+      inversion HSubB as [x HsB]; inversion HsB; subst; try orthoax_inv PTypHd2.
+      apply PTypHd3; auto.
+    + now apply HNotTL.
+Admitted.
+
+Lemma foo : forall A, TopLike A -> forall e1, exists e2, and_coercion A e1 = inl e2.
+  intros A T. induction T; simpl; intros.
+  exists (STUnit _). auto.
+  destruct (IHT1 e1). destruct (IHT2 e1). rewrite H, H0.
+  eauto.
+  destruct (IHT e1). rewrite H.
+  exists (STLam _ x). auto.
+  eauto.
+  Defined.
+
+Lemma same_coercion : forall A, TopLike A -> forall e1 e2, and_coercion A e1 = and_coercion A e2.
+  intros A T. induction T; simpl; intros; auto. rewrite (IHT1 e1 e2). rewrite (IHT2 e1 e2).
+  pose (foo _ T1 e2). destruct e. rewrite H. pose (foo _ T2 e2). destruct e. rewrite H0. auto.
+  rewrite (IHT e1 e2). auto.
+Defined.
+
+(* Coercive subtyping is coeherent: Lemma 3 *)
+
+Lemma sub_coherent :
+  forall {A Gamma}, WFTyp Gamma A ->
+           forall {B}, WFTyp Gamma B ->
+                  forall {C1}, sub A B C1 ->
+                          forall {C2}, sub A B C2 -> C1 = C2.
+Proof.
+  intros.
+  generalize dependent C2.
+  generalize dependent Gamma.
+  (* Case: Int <: Int *)
+  induction H1; intros.
+  - inversion H2. 
+    reflexivity.
+  (* Case: Fun t1 t2 <: Fun t3 t4 *)
+  - inversion H. inversion H0. inversion H2.
+    assert (c2 = c3). apply IHsub2 with (Gamma := Gamma); auto.
+    assert (c1 = c0). apply IHsub1 with (Gamma := Gamma); auto.
+    now subst.
+  (* Case: t <: And t1 t2 *) 
+  - inversion H2; inversion H0; subst.
+    assert (c1 = c0) by (apply IHsub1 with (Gamma := Gamma); auto).
+    assert (c2 = c3) by (apply IHsub2 with (Gamma := Gamma); auto).
+    now subst.
+    now subst.
+    now subst.
+  (* different coercion case*)
+  - inversion H2; subst.
+    inversion H4; subst.
+    inversion H.
+    assert (c = c0). apply IHsub with (Gamma := Gamma); auto.
+    now subst.
+    destruct (toplike_dec t0).
+    erewrite same_coercion.
+    reflexivity.
+    apply t3.
+    assert (HSub : Sub (And t1 t2) t0) by (apply sand2; unfold Sub; eauto).
+    assert (Ha := uniquesub _ t1 t2 t0 H7 H9 n H10 HSub).
+    exfalso; apply Ha.
+    split; unfold Sub; eauto.
+    inversion H.
+  - inversion H2; subst.
+    inversion H4; subst.
+    inversion H.
+    destruct (toplike_dec t0).
+    erewrite same_coercion.
+    reflexivity.
+    apply t3.    
+    assert (HSub : Sub (And t1 t2) t0) by (apply sand3; unfold Sub; eauto).
+    assert (Ha := uniquesub _ t1 t2 t0 H7 H9 n H10 HSub).
+    exfalso; apply Ha.
+    split; unfold Sub; eauto.
+    assert (c = c0). apply IHsub with (Gamma := Gamma); auto.
+    now subst.
+    now subst.
+  - now inversion H2.
+  - inversion H2; subst.
+    inversion H3; subst.
+    inversion H4; subst.
+    pick_fresh x.
+    assert (Ha : (open_typ_term c (STFVarT x)) = (open_typ_term c0 (STFVarT x))).
+    assert (ty := Top).
+    eapply H0 with (Gamma := extend x (TyDis d) Gamma).
+    not_in_L x.
+    apply H8.
+    not_in_L x.
+    apply H10.
+    not_in_L x.
+    apply H12.
+    not_in_L x.
+    assert (c = c0).
+    eapply open_typ_term_app_eq with (x := x) (n := 0).
+    not_in_L x.
+    not_in_L x.
+    apply Ha.
+    now subst.
+  - inversion H2.
+    inversion H4.
+    inversion H4.
+    now subst.    
+Qed.
+
+(*
+End ExtendedSub.
+
+Module Extended
+       (Import VarTyp : UsualDecidableTypeFull)
+       (Import set : MSetInterface.S).
+
+Require Import Extended_infrastructure.
+Module Infrastructure := Infrastructure(VarTyp)(set).
+Export Infrastructure.
+
+Module ExtendedSub := ExtendedSub(VarTyp)(set).
+Import ExtendedSub.
+ *)
+
+(* Typing lemmas *)
+
+Lemma typing_wf_source_alg:
+  forall Gamma t T E dir, has_type_source_alg Gamma t dir T E -> WFTyp Gamma T.
+Proof.
+  intros Gamma t dir T E H.
+  induction H; auto.
+  - inversion IHhas_type_source_alg1; assumption.
+  - inversion IHhas_type_source_alg; subst.
+    apply open_body_wf_type with (d := d); auto.
+    unfold body_wf_typ; eauto.
+  - pick_fresh x.
+    assert (Ha : not (M.In x L)) by (not_in_L x).
+    apply WFFun.
+    assumption.
+    apply H0 in Ha.
+    rewrite <- app_nil_l with (l := Gamma).
+    eapply wf_strengthen_source with (z := x).
+    not_in_L x.
+    rewrite app_nil_l; apply Ha.
+  - apply_fresh WFForAll as x.
+    apply H1.
+    not_in_L x.
+    auto.
+Qed.
+
+Lemma type_correct_alg_terms : forall Gamma E ty e dir, has_type_source_alg Gamma E dir ty e -> PTerm E.
+Proof.
+  intros.
+  induction H; auto.
+  - apply PTerm_TApp.
+    auto.
+    now apply wf_gives_types_source in H.
+  - apply_fresh PTerm_Lam as x; auto.
+    apply H0; not_in_L x.
+  - apply_fresh PTerm_TLam as x.
+    apply H1; not_in_L x.
+Qed.
+
+
+Lemma typing_alg_wf_env :
+  forall Gamma E dir ty e, has_type_source_alg Gamma E dir ty e -> WFEnv Gamma.
+Proof.
+  intros.
+  induction H; auto.
+  - pick_fresh x;
+    assert (Ha: not (In x L)) by not_in_L x;
+    pose (H0 _ Ha) as HInv;
+    inversion HInv; auto.
+  - pick_fresh x.
+    assert (Ha : not (In x L)) by not_in_L x.
+    apply H1 in Ha.
+    now inversion Ha.
+Qed.
+  
+(* Ignoring the generated expressions + smart constructors *)
+
+Definition has_ty Gamma e d t := exists E, has_type_source_alg Gamma e d t E.
+
+(* Uniqueness *)
+
+Definition almost_unique (A B : PTyp) (d : Dir) : Prop := 
+  match d with
+    | Inf => A = B
+    | Chk => True (* Is this result useful for checking: exists C, Sub C A /\ Sub C B*)
+  end.
+
+Lemma typ_unique : forall Gamma e d t1 E1, has_type_source_alg Gamma e d t1 E1 -> forall t2 E2, has_type_source_alg Gamma e d t2 E2 -> almost_unique t1 t2 d.
+intros Gamma e d t1 E1 H.
+induction H; intros; unfold almost_unique; auto.
+(* case Var *)
+- inversion H2; subst.
+  assert (Ha : TermV ty = TermV t2).
+  erewrite ok_unique_type with (x0 := x).
+  reflexivity.
+  apply wfenv_to_ok in H4.
+  apply H4.
+  apply (conj H5 H0).
+  decide equality.
+  now inversion Ha.
+(* case Lit *)
+- inversion H0. auto.
+(* case App *)
+- inversion H1.
+  apply IHhas_type_source_alg1 in H5. simpl in H5.
+  apply IHhas_type_source_alg2 in H6.
+  injection H5. intros. auto.
+(* Case Merge *)
+- inversion H2.
+  apply IHhas_type_source_alg1 in H5.
+  apply IHhas_type_source_alg2 in H7.
+  rewrite H5. rewrite H7. auto.
+(* Case Ann *)
+- inversion H0. auto.
+(* Case TApp *)
+- inversion H2; subst.
+  apply IHhas_type_source_alg in H7.
+  injection H7; intros.
+  now subst.
+Qed.
+
+(* Theorem 5. Type inference always gives unique types *)
+
+Lemma typ_inf_unique : forall {Gamma e t1 t2 E1 E2}, has_type_source_alg Gamma e Inf t1 E1 -> has_type_source_alg Gamma e Inf t2 E2 -> t1 = t2.
+intros.
+pose (@typ_unique _ _ _ _ _ H _ _ H0). simpl in a. auto.
+Qed.
+
+(* Theorem 6. *)
+Lemma typ_coherence : forall Gamma e d t E1, has_type_source_alg Gamma e d t E1 -> forall E2, has_type_source_alg Gamma e d t E2 -> E1 = E2.
+intros Gamma e d t E1 H.
+induction H; intros.
+(* case PFVar *)
+- inversion H2; reflexivity. 
+(* case STLit *)
+- inversion H0; reflexivity.
+(* Case App *)
+- inversion H1.
+  assert (Fun A B = Fun A0 B).
+  apply (typ_inf_unique H H5). injection H9. intros.
+  rewrite <- H9 in H5. rewrite <- H10 in H6.
+  apply IHhas_type_source_alg1 in H5. 
+  apply IHhas_type_source_alg2 in H6.
+  rewrite H5. rewrite H6. auto.
+(* Case Merge *)
+- inversion H2.
+  apply IHhas_type_source_alg1 in H8.
+  apply IHhas_type_source_alg2 in H9.
+  rewrite H8. rewrite H9. auto.
+(* Case Ann *)
+- inversion H0.
+  apply IHhas_type_source_alg in H3. auto.
+(* Case TApp *)
+- inversion H2; subst.
+  assert (Ha : ForAll d ty = ForAll d0 ty0).
+  eapply typ_inf_unique.
+  apply H0.
+  apply H8.
+  rewrite <- Ha in H8.
+  apply IHhas_type_source_alg in H8.
+  now subst.
+(* Case Lam *)
+- inversion H2; subst.
+  apply f_equal.
+  pick_fresh x.
+  assert (Ha1: not (M.In x L0)) by (not_in_L x).
+  apply H7 in Ha1.
+  apply H0 in Ha1.
+  assert (HNotE : not (In x (fv E))) by (not_in_L x).
+  assert (HNotF : not (In x (fv E0))) by (not_in_L x).
+  apply (open_app_eq _ _ _ _ HNotE HNotF Ha1).
+  not_in_L x.
+  inversion H3. 
+(* ATySub *)
+- inversion H2.
+  subst.
+  inversion H.
+  assert (A = A0).
+  apply (typ_inf_unique H H3).
+  subst.
+  apply IHhas_type_source_alg in H3.
+  subst.
+  assert (WFTyp Gamma A0). now apply typing_wf_source_alg in H.
+  assert (WFTyp Gamma B). assumption.
+  assert (C = C0).
+  apply (sub_coherent H3 H6 H0 H4).
+  subst; reflexivity.
+  subst; inversion H.
+(* Case TLam *)
+- inversion H2; subst.
+  inversion H3.
+  apply f_equal.
+  pick_fresh x.
+  apply open_typ_term_app_eq with (E := E) (F := E0) (x := x) (n := 0).
+  not_in_L x.
+  not_in_L x.
+  apply H1.
+  not_in_L x.
+  apply H8.
+  not_in_L x.
+Qed.
+
+Lemma coercions_produce_terms :
+  forall E A B, sub A B E -> STTerm E.
+Proof.
+  intros.
+  induction H.
+  (* Case SInt *)
+  - apply_fresh STTerm_Lam as x; cbn; auto.
+  (* Case SFun *)
+  - apply_fresh STTerm_Lam as x; cbn.
+    apply_fresh STTerm_Lam as y; cbn.
+    apply STTerm_App.
+    repeat rewrite <- open_rec_term; assumption.
+    apply STTerm_App.
+    apply STTerm_Var.
+    apply STTerm_App; [ repeat rewrite <- open_rec_term; auto | apply STTerm_Var ].
+  (* Case SAnd1 *)
+  - apply_fresh STTerm_Lam as x; cbn.
+    apply STTerm_Pair.
+    apply STTerm_App; repeat rewrite <- open_rec_term; auto.
+    rewrite <- open_rec_term; auto.
+  (* Case SAnd2 *)
+  - apply_fresh STTerm_Lam as x; cbn.
+    apply STTerm_App; auto.
+    rewrite <- open_rec_term; auto.    
+  (* Case SAnd3 *)
+  - apply_fresh STTerm_Lam as x; cbn.
+    apply STTerm_App; auto.
+    rewrite <- open_rec_term; auto.
+  (* Case SVar *)
+  - apply_fresh STTerm_Lam as x; cbn; auto.
+  (* Case SForAll *)
+  - apply_fresh STTerm_Lam as x; cbn.
+    apply_fresh STTerm_TLam as y; cbn.
+    apply STTerm_App; auto.
+    assert (Ha : not (In y L)) by (not_in_L y).
+    apply H0 in Ha.
+    rewrite open_comm_open_typ_term.
+    rewrite <- open_rec_term; auto.
+Qed.
+
+Hint Resolve coercions_produce_terms.
+
+
+(* Subtyping rules produce type-correct coercions: Lemma 1 *)
+Lemma type_correct_coercions :
+  forall Gamma A B E, sub A B E ->
+             WFEnv Gamma ->
+             WFTyp Gamma A ->
+             WFTyp Gamma B ->
+             has_type_st (∥ Gamma ∥) E (STFun (|A|) (|B|)) .
+Proof.
+  intros.
+  generalize dependent Gamma.
+  induction H; intros.
+  (* Case SInt *)
+  - simpl.
+    remember (∥ Gamma ∥).
+    apply_fresh STTyLam as x; cbn; auto.
+    apply STTyVar; auto.
+    apply WFType_Int; auto.
+    apply Ok_push; auto.
+    subst; auto.
+    apply wfenv_to_ok in H0; auto.
+    not_in_L x.
+    apply Ok_push; auto.
+    subst; auto.
+    not_in_L x.
+    left; simpl; auto.
+    apply WFType_Int.
+    subst; auto.
+  (* Case SFun *)
+  - inversion H2; inversion H3.
+    subst.
+    remember (∥ Gamma ∥).
+    apply_fresh STTyLam as x; cbn.
+    apply_fresh STTyLam as y; cbn.
+    apply STTyApp with (A := (| o2 |)).
+    rewrite <- open_rec_term.
+    rewrite <- open_rec_term.
+    repeat apply typing_weaken_extend.
+    subst; apply (IHsub2 _ H1 H8 H13).
+    not_in_L x.
+    not_in_L y.
+    not_in_L x.
+    now apply coercions_produce_terms in H0.
+    rewrite <- open_rec_term.
+    now apply coercions_produce_terms in H0.
+    now apply coercions_produce_terms in H0.
+    apply STTyApp with (A := (| o1 |)).
+    apply STTyVar.
+    repeat apply wf_weaken_extend.
+    apply WFType_Fun.
+    subst; now apply WFTyp_to_WFType.
+    subst; now apply WFTyp_to_WFType.
+    not_in_L x.
+    not_in_L y.
+    not_in_L x.
+    apply Ok_push.
+    apply Ok_push.
+    subst; auto.
+    not_in_L x.
+    not_in_L y.
+    not_in_L x.
+    right; left; auto.
+    rewrite <- open_rec_term.
+    rewrite <- open_rec_term.
+    eapply STTyApp.
+    repeat apply typing_weaken_extend.
+    subst; apply IHsub1; auto.
+    not_in_L x.
+    not_in_L y.
+    not_in_L x.
+    apply STTyVar.
+    repeat apply wf_weaken_extend.
+    inversion H3.
+    subst; now apply WFTyp_to_WFType.
+    not_in_L x.
+    not_in_L y.
+    not_in_L x.
+    apply Ok_push.
+    apply Ok_push.
+    subst; auto.
+    not_in_L x.
+    not_in_L y.
+    not_in_L x.
+    left; auto.    
+    now apply coercions_produce_terms in H.
+    rewrite <- open_rec_term.
+    now apply coercions_produce_terms in H.
+    now apply coercions_produce_terms in H.
+    apply wf_weaken_extend.
+    subst; now apply WFTyp_to_WFType.
+    not_in_L x.
+    apply WFType_Fun; subst; now apply WFTyp_to_WFType.
+  - remember (∥ Gamma ∥).
+    inversion H3.
+    apply_fresh STTyLam as x; cbn.
+    apply STTyPair.
+    + rewrite <- open_rec_term.
+      apply STTyApp with (A := (| t0 |)).
+      apply typing_weaken_extend.
+      subst; apply IHsub1; auto.
+      not_in_L x.
+      apply STTyVar.
+      apply wf_weaken_extend.
+      subst; now apply WFTyp_to_WFType.
+      not_in_L x.
+      apply Ok_push.
+      subst; auto.
+      not_in_L x.
+      left; auto.
+      now apply coercions_produce_terms in H.
+    + rewrite <- open_rec_term.
+      apply STTyApp with (A := (| t0 |)).
+      apply typing_weaken_extend.
+      subst; apply IHsub2; auto.
+      not_in_L x.
+      apply STTyVar.
+      apply wf_weaken_extend.
+      subst; now apply WFTyp_to_WFType.
+      not_in_L x.
+      apply Ok_push.
+      subst; auto.
+      not_in_L x.
+      left; auto.
+      now apply coercions_produce_terms in H0.
+    + subst; now apply WFTyp_to_WFType.
+  - remember (∥ Gamma ∥).
+    inversion H2.
+    apply_fresh STTyLam as x; cbn.
+    rewrite <- open_rec_term.
+    apply STTyApp with (A := (| t1 |)).
+    apply typing_weaken_extend.
+    subst; apply IHsub; auto.
+    not_in_L x.
+    apply STTyProj1 with (B := (| t2 |)).
+    apply STTyVar.
+    apply wf_weaken_extend.
+    apply WFType_Tuple; subst; now apply WFTyp_to_WFType.
+    not_in_L x.
+    apply Ok_push. subst; auto. not_in_L x.
+    left; auto.
+    now apply coercions_produce_terms in H.
+    subst; apply WFType_Tuple; now apply WFTyp_to_WFType.
+  - remember (∥ Gamma ∥).
+    inversion H2.
+    apply_fresh STTyLam as x; cbn.
+    rewrite <- open_rec_term.
+    apply STTyApp with (A := (| t2 |)).
+    apply typing_weaken_extend.
+    subst; apply IHsub; auto.
+    not_in_L x.
+    apply STTyProj2 with (A := (| t1 |)).
+    apply STTyVar.
+    apply wf_weaken_extend.
+    apply WFType_Tuple; subst; now apply WFTyp_to_WFType.
+    not_in_L x.
+    apply Ok_push. subst; auto. not_in_L x.
+    left; auto.
+    now apply coercions_produce_terms in H.
+    subst; apply WFType_Tuple; now apply WFTyp_to_WFType.
+  - remember (∥ Gamma ∥).
+    apply_fresh STTyLam as x.
+    unfold open; simpl.
+    apply STTyVar.
+    apply wf_weaken_extend.
+    subst; now apply WFTyp_to_WFType in H1.
+    not_in_L x.
+    apply Ok_push.
+    subst; auto.
+    not_in_L x.
+    left; auto.
+    subst; now apply WFTyp_to_WFType in H1.    
+  - remember (∥ Gamma ∥).
+    inversion H2.
+    inversion H3.
+    apply_fresh STTyLam as x.
+    unfold open; simpl.
+    apply_fresh STTyTLam as y.
+    unfold open_typ_term; simpl.
+    apply STTyApp with (A := (open_typ (| t1 |) (STFVarT y))).
+    rewrite open_comm_open_typ_term.
+    rewrite <- open_rec_term.
+    unfold open_typ; simpl.
+    unfold open_typ_source in H0; simpl in H0.
+    subst.
+    change (extend y (TyVar STyp)
+                   (extend x (TermVar STyp (STForAll (| t1 |))) (∥ Gamma ∥))) with
+    (∥ (extend y (TyDis d)
+               (extend x (TermV (ForAll d t1)) Gamma)) ∥).
+    change (STFVarT y) with (| PFVarT y |).
+    rewrite <- open_rec_typ_eq_source.
+    rewrite <- open_rec_typ_eq_source.
+    apply H0.
+    not_in_L y.
+    apply WFPushV.
+    apply WFPushT.
+    auto.
+    not_in_L x.
+    not_in_L y.
+    simpl.
+    unfold not; intro HH.
+    apply MSetProperties.Dec.F.add_iff in HH.
+    destruct HH; subst.
+    not_in_L y.
+    exfalso; apply H25; now apply MSetProperties.Dec.F.singleton_2.
+    not_in_L y.
+    unfold extend.
+    apply wf_weaken_source.
+    apply H7.
+    not_in_L y.
+    apply WFPushV.
+    apply WFPushT.
+    auto.
+    not_in_L x.
+    not_in_L y.
+    simpl.
+    unfold not; intro HH.
+    apply MSetProperties.Dec.F.add_iff in HH.
+    destruct HH; subst.
+    not_in_L y.
+    exfalso; apply H25; now apply MSetProperties.Dec.F.singleton_2.
+    not_in_L y.
+    apply wf_weaken_source.
+    apply H12.
+    not_in_L y.
+    apply WFPushV.
+    apply WFPushT.
+    auto.
+    not_in_L x.
+    not_in_L y.
+    not_in_L y.
+    not_in_L x.
+    assert (Ha : not (In y L)) by not_in_L y.
+    apply H in Ha.
+    now apply coercions_produce_terms in Ha.
+    apply STTyTApp.
+    apply WFType_Var.
+    apply Ok_push.
+    apply Ok_push.
+    subst; auto.
+    not_in_L x.
+    unfold extend; not_in_L y.
+    not_in_L x.
+    left; auto.
+    apply STTyVar.
+    apply WFTyp_to_WFType in H2.
+    repeat apply wf_weaken_extend.
+    subst; apply H2.
+    not_in_L x.
+    unfold extend; not_in_L y.
+    not_in_L x.
+    apply Ok_push.
+    apply Ok_push.
+    subst; auto.
+    not_in_L x.
+    unfold extend; not_in_L y.
+    not_in_L x.
+    right; left; auto.
+    subst; now apply WFTyp_to_WFType in H2.
+    subst; inversion H8.
+    subst.
+
+
+    inversion H2; inversion H3; subst.
+    inversion H14.
+    inversion H9.
+    inversion H12.
+    apply_fresh STTyLam as x.
+    unfold open; simpl.
+    apply_fresh STTyTLam as y.
+    unfold open_typ_term; simpl.
+    apply STTyApp with (A := (open_typ (| t1 |) (STFVarT y))).
+    rewrite open_comm_open_typ_term.
+    rewrite <- open_rec_term.
+    unfold open_typ; simpl.
+    unfold open_typ_source in H0; simpl in H0.
+    subst.
+    change (extend y (TyVar STyp)
+                   (extend x (TermVar STyp (STForAll (| t1 |))) (∥ Gamma ∥))) with
+    (∥ (extend y (TyDis Bot)
+               (extend x (TermV (ForAll Bot t1)) Gamma)) ∥).
+    change (STFVarT y) with (| PFVarT y |).
+    rewrite <- open_rec_typ_eq_source.
+    rewrite <- open_rec_typ_eq_source.
+    apply H0.
+    not_in_L y.
+    apply WFPushV.
+    apply WFPushT.
+    auto.
+    not_in_L x.
+    not_in_L y.
+    inversion H8.
+    simpl.
+    unfold not; intro HH.
+    apply MSetProperties.Dec.F.add_iff in HH.
+    destruct HH; subst.
+    not_in_L y.
+    exfalso; apply H14; now apply MSetProperties.Dec.F.singleton_2.
+    not_in_L y.
+    unfold extend.
+    apply wf_weaken_source.
+    apply H6.
+    not_in_L y.
+    apply WFPushV.
+    apply WFPushT.
+    auto.
+    not_in_L x.
+    not_in_L y.
+    inversion H8.
+    simpl.
+    unfold not; intro HH.
+    apply MSetProperties.Dec.F.add_iff in HH.
+    destruct HH; subst.
+    not_in_L y.
+    exfalso; apply H14; now apply MSetProperties.Dec.F.singleton_2.
+    not_in_L y.
+    apply wf_weaken_source.
+    apply H10.
+    not_in_L y.
+    apply WFPushV.
+    apply WFPushT.
+    auto.
+    not_in_L x.
+    unfold not; intros HH; inversion HH.
+    not_in_L y.
+    not_in_L y.
+    not_in_L x.
+    assert (Ha : not (In y L)) by not_in_L y.
+    apply H in Ha.
+    now apply coercions_produce_terms in Ha.
+    apply STTyTApp.
+    apply WFType_Var.
+    apply Ok_push.
+    apply Ok_push.
+    subst; auto.
+    not_in_L x.
+    (* TODO add this to not_in_L *)
+    unfold conv_context in H4; rewrite <- dom_map_id in H4; contradiction.
+    unfold extend; not_in_L y.
+    not_in_L x.
+    unfold conv_context in H8; rewrite <- dom_map_id in H8; contradiction.
+    left; auto.
+    apply STTyVar.
+    apply WFTyp_to_WFType in H2.
+    repeat apply wf_weaken_extend.
+    subst; apply H2.
+    not_in_L x.
+    unfold conv_context in H4; rewrite <- dom_map_id in H4; contradiction.
+    unfold extend; not_in_L y.
+    not_in_L x.
+    unfold conv_context in H8; rewrite <- dom_map_id in H8; contradiction.
+    apply Ok_push.
+    apply Ok_push.
+    subst; auto.
+    not_in_L x.
+    unfold conv_context in H4; rewrite <- dom_map_id in H4; contradiction.
+    unfold extend; not_in_L y.
+    not_in_L x.
+    unfold conv_context in H8; rewrite <- dom_map_id in H8; contradiction.
+    right; left; auto.
+    subst; now apply WFTyp_to_WFType in H2.
+Qed.
+  
+(* Type preservation: Theorem 1 *)
+Lemma type_preservation :
+  forall x ty dir E (Gamma : context TyEnvSource) (H : has_type_source_alg Gamma x dir ty E),
+  has_type_st (∥ Gamma ∥) E (|ty|).
+Proof.
+  intros.
+  induction H; subst; auto.
+  (* TyVar *)
+  - apply STTyVar.
+    now apply WFTyp_to_WFType.
+    auto.
+    now apply in_persists in H0.
+  (* TyApp *)
+  - simpl in *.
+    apply STTyApp with (A := |A|).
+    assumption.
+    assumption.
+  (* TyMerge *)
+  - simpl; apply STTyPair; assumption.
+  (* TyTApp *)
+  - simpl in *.
+    unfold open_typ_source; rewrite open_rec_typ_eq_source.
+    apply STTyTApp.
+    now apply WFTyp_to_WFType.
+    apply IHhas_type_source_alg.
+  (* TyLam *)
+  - simpl.
+    apply_fresh STTyLam as x.
+    unfold open; simpl.
+    assert (Ha : not (M.In x L)).
+    not_in_L x.
+    apply H0 in Ha.
+    simpl in *.
+    unfold extend.
+    simpl.
+    apply Ha.
+    now apply WFTyp_to_WFType.
+  (* ATySub *)
+  - apply STTyApp with (|A|).
+    apply type_correct_coercions.
+    assumption.
+    now apply typing_alg_wf_env in H.
+    now apply typing_wf_source_alg in H.
+    assumption.
+    assumption.
+  (* ATyTLam *)
+  - simpl; apply_fresh STTyTLam as x.
+    simpl in *.
+    unfold open_typ.
+    change (STFVarT x) with (| PFVarT x |).
+    rewrite <- open_rec_typ_eq_source.
+    apply H1.
+    not_in_L x.
+  (* ATyTLamBot *)
+  - simpl; apply_fresh STTyTLam as x.
+    simpl in *.
+    unfold open_typ.
+    change (STFVarT x) with (| PFVarT x |).
+    rewrite <- open_rec_typ_eq_source.
+    apply H0.
+    not_in_L x.
+Qed.
+
+End Extended.
